@prefix : <http://w3id.org/polifonia/ontology/jams/> .
@prefix dc: <http://purl.org/dc/elements/1.1/> .
@prefix mm: <https://w3id.org/polifonia/ontology/music-meta/> .
@prefix mp: <https://w3id.org/polifonia/ontology/music-projection/> .
@prefix mr: <https://w3id.org/polifonia/ontology/music-representation/> .
@prefix owl: <http://www.w3.org/2002/07/owl#> .
@prefix rdf: <http://www.w3.org/1999/02/22-rdf-syntax-ns#> .
@prefix xml: <http://www.w3.org/XML/1998/namespace> .
@prefix xsd: <http://www.w3.org/2001/XMLSchema#> .
@prefix core: <https://w3id.org/polifonia/ontology/core/> .
@prefix prov: <http://www.w3.org/ns/prov#> .
@prefix rdfs: <http://www.w3.org/2000/01/rdf-schema#> .
@prefix skos: <http://www.w3.org/2004/02/skos/core#> .
@prefix terms: <http://purl.org/dc/terms/> .
@prefix polifonia-res: <http://w3id.org/polifonia/resource/> .
@prefix cpannotationschema: <http://www.ontologydesignpatterns.org/schemas/cpannotationschema.owl#> .
@base <http://w3id.org/polifonia/ontology/jams/> .

<http://w3id.org/polifonia/ontology/jams/> rdf:type owl:Ontology ;
                                            owl:versionIRI <http://w3id.org/polifonia/ontology/jams/1.0/> ;
                                            owl:imports mp: ,
                                                        mr: ;
                                            dc:creator "Albert Merono Penuela"@en ,
                                                       "Andrea Poltronieri"@en ,
                                                       "Jacpo de Berardinis" ,
                                                       "Valentina Presutti"@en ;
                                            dc:license <https://creativecommons.org/licenses/by-sa/4.0/> ;
                                            terms:license <https://creativecommons.org/licenses/by-sa/4.0/> ;
                                            rdfs:comment """An ontology for modelling a JAMS file containing different types of musical annotations. 
In particular, this ontology focuses on the Chord Annotations contained in the JAMS file and their attributes."""@en ;
                                            rdfs:label "JAMS Ontology"@en ;
                                            owl:versionInfo "1.0"@en .

#################################################################
#    Annotation properties
#################################################################

###  http://purl.org/dc/elements/1.1/creator
dc:creator rdf:type owl:AnnotationProperty .


###  http://purl.org/dc/elements/1.1/license
dc:license rdf:type owl:AnnotationProperty .


###  http://purl.org/dc/elements/1.1/title
dc:title rdf:type owl:AnnotationProperty .


###  http://purl.org/dc/terms/contributor
terms:contributor rdf:type owl:AnnotationProperty .


###  http://purl.org/dc/terms/creator
terms:creator rdf:type owl:AnnotationProperty .


###  http://purl.org/dc/terms/description
terms:description rdf:type owl:AnnotationProperty .


###  http://purl.org/dc/terms/license
terms:license rdf:type owl:AnnotationProperty .


###  http://purl.org/dc/terms/title
terms:title rdf:type owl:AnnotationProperty .


#################################################################
#    Object Properties
#################################################################

###  http://w3id.org/polifonia/ontology/jams/hasAnnotationType
:hasAnnotationType rdf:type owl:ObjectProperty ;
                   owl:inverseOf :isAnnotationTypeOf ;
                   rdf:type owl:FunctionalProperty ;
                   rdfs:domain :JAMSAnnotation ;
                   rdfs:range :AnnotationType ;
                   owl:propertyDisjointWith :hasAnnotator ,
                                            :hasAnnotatorType ,
                                            :hasChordSubject ,
                                            :hasFormat ,
                                            :hasJAMSAnnotation ,
                                            :hasMusicTimeDuration ,
                                            :hasMusicTimeIndex ,
                                            :hasMusicTimeIndexComponent ,
                                            :hasMusicTimeInterval ,
                                            :hasSubject ,
                                            :hasValueType ,
                                            :includesObservation ,
                                            :isAnnotationTypeOf ,
                                            :isAnnotatorOf ,
                                            :isAnnotatorTypeOf ,
                                            :isMusicTimeDurationOf ,
                                            :isMusicTimeIndexComponentOf ,
                                            :isMusicTimeIndexOf ,
                                            :isMusicTimeIntervalOf ,
                                            :isObservationOf ,
                                            :isValueTypeOf ;
                   rdfs:comment "Links an Annotation to its AnnotationType, defining the content of the annotations (e.g. chords, key, patterns, etc.):"@en ;
                   rdfs:label "Has Annotation Type"@en .


###  http://w3id.org/polifonia/ontology/jams/hasAnnotator
:hasAnnotator rdf:type owl:ObjectProperty ;
              owl:inverseOf :isAnnotatorOf ;
              rdfs:domain :JAMSAnnotation ;
              owl:propertyDisjointWith :hasAnnotatorType ,
                                       :hasJAMSAnnotation ,
                                       :hasMusicTimeDuration ,
                                       :hasMusicTimeIndex ,
                                       :hasMusicTimeIndexComponent ,
                                       :hasMusicTimeInterval ,
                                       :hasSubject ,
                                       :hasValueType ,
                                       :includesObservation ,
                                       :isAnnotatorOf ,
                                       :isAnnotatorTypeOf ,
                                       :isJAMSAnnotationOf ,
                                       :isMusicTimeDurationOf ,
                                       :isMusicTimeIndexComponentOf ,
                                       :isMusicTimeIndexOf ,
                                       :isObservationOf ,
                                       :isValueTypeOf ;
              rdfs:comment "Links a JAMS annotation to the Annotator the annotated the JAMS."@en ;
              rdfs:label "Has Annotator"@en .


###  http://w3id.org/polifonia/ontology/jams/hasAnnotatorType
:hasAnnotatorType rdf:type owl:ObjectProperty ;
                  owl:inverseOf :isAnnotatorTypeOf ;
                  rdf:type owl:FunctionalProperty ;
                  rdfs:range :AnnotatorType ;
                  owl:propertyDisjointWith :hasChordSubject ,
                                           :hasFormat ,
                                           :hasJAMSAnnotation ,
                                           :hasMusicTimeDuration ,
                                           :hasMusicTimeIndex ,
                                           :hasMusicTimeIndexComponent ,
                                           :hasMusicTimeInterval ,
                                           :hasSubject ,
                                           :hasValueType ,
                                           :includesObservation ,
                                           :isAnnotationTypeOf ,
                                           :isAnnotatorOf ,
                                           :isAnnotatorTypeOf ,
                                           :isJAMSAnnotationOf ,
                                           :isMusicTimeDurationOf ,
                                           :isMusicTimeIndexComponentOf ,
                                           :isMusicTimeIndexOf ,
                                           :isMusicTimeIntervalOf ,
                                           :isObservationOf ,
                                           :isValueTypeOf ;
                  rdfs:comment "Links the Annotator class to its Annotator Type, describing how the JAMS annotations were generated."@en ;
                  rdfs:label "Has Annotator Type"@en .


###  http://w3id.org/polifonia/ontology/jams/hasChordSubject
:hasChordSubject rdf:type owl:ObjectProperty ;
                 rdfs:subPropertyOf :hasSubject ;
                 rdf:type owl:FunctionalProperty ;
                 rdfs:domain :JAMSObservation ;
                 rdfs:range mp:Chord ;
                 owl:propertyDisjointWith :hasFormat ,
                                          :hasJAMSAnnotation ,
                                          :hasMusicTimeDuration ,
                                          :hasMusicTimeIndex ,
                                          :hasMusicTimeIndexComponent ,
                                          :hasMusicTimeInterval ,
                                          :hasValueType ,
                                          :includesObservation ,
                                          :isAnnotationTypeOf ,
                                          :isAnnotatorOf ,
                                          :isAnnotatorTypeOf ,
                                          :isMusicTimeDurationOf ,
                                          :isMusicTimeIndexComponentOf ,
                                          :isMusicTimeIndexOf ,
                                          :isMusicTimeIntervalOf ,
                                          :isObservationOf ,
                                          :isValueTypeOf ;
                 rdfs:comment "Links a JAMSObservation to the observation value, in the case the value is a musical chord."@en ;
                 rdfs:label "Has Chord Subject"@en .


###  http://w3id.org/polifonia/ontology/jams/hasEndMusicTimeIndex
:hasEndMusicTimeIndex rdf:type owl:ObjectProperty ;
                      rdfs:subPropertyOf :hasMusicTimeIndex ,
                                         [ owl:inverseOf :isMusicTimeIndexOf
                                         ] ;
                      rdfs:domain :MusicTimeInterval ;
                      rdfs:range :MusicTimeIndex ;
                      rdfs:comment "Subproperty of jasMusicTimeIndex. It links a MusicTimeInterval to its MusicTimeIndex, defining the end point of validity of an observation/annotation time interval."@en ;
                      rdfs:label "Has End Music Time Index"@en .


###  http://w3id.org/polifonia/ontology/jams/hasFormat
:hasFormat rdf:type owl:ObjectProperty ;
           rdfs:subPropertyOf owl:topObjectProperty ;
           rdf:type owl:FunctionalProperty ;
           rdfs:domain :File ;
           rdfs:range :Format ;
           owl:propertyDisjointWith :hasJAMSAnnotation ,
                                    :hasMusicTimeDuration ,
                                    :hasMusicTimeIndex ,
                                    :hasMusicTimeIndexComponent ,
                                    :hasMusicTimeInterval ,
                                    :hasSubject ,
                                    :hasValueType ,
                                    :includesObservation ,
                                    :isAnnotationTypeOf ,
                                    :isAnnotatorOf ,
                                    :isJAMSAnnotationOf ,
                                    :isMusicTimeDurationOf ,
                                    :isMusicTimeIndexComponentOf ,
                                    :isMusicTimeIndexOf ,
                                    :isObservationOf ,
                                    :isValueTypeOf ;
           rdfs:comment "Links a File to its Format, defining the type of the file."@en ;
           rdfs:label "Has Format"@en .


###  http://w3id.org/polifonia/ontology/jams/hasJAMSAnnotation
:hasJAMSAnnotation rdf:type owl:ObjectProperty ;
                   owl:inverseOf :isJAMSAnnotationOf ;
                   rdf:type owl:InverseFunctionalProperty ;
                   rdfs:domain mr:MusicContent ;
                   rdfs:range :JAMSAnnotation ;
                   owl:propertyDisjointWith :hasMusicTimeDuration ,
                                            :hasMusicTimeIndex ,
                                            :hasMusicTimeIndexComponent ,
                                            :hasMusicTimeInterval ,
                                            :hasSubject ,
                                            :hasValueType ,
                                            :includesObservation ,
                                            :isAnnotationTypeOf ,
                                            :isAnnotatorOf ,
                                            :isAnnotatorTypeOf ,
                                            :isJAMSAnnotationOf ,
                                            :isMusicTimeDurationOf ,
                                            :isMusicTimeIndexComponentOf ,
                                            :isMusicTimeIntervalOf ,
                                            :isObservationOf ,
                                            :isValueTypeOf ;
                   rdfs:comment "Relates a Score or a Recording to the JAMS annotation describing the track."@en ;
                   rdfs:label "Has JAMS Annotation"@en .


###  http://w3id.org/polifonia/ontology/jams/hasMusicTimeDuration
:hasMusicTimeDuration rdf:type owl:ObjectProperty ;
                      owl:inverseOf :isMusicTimeDurationOf ;
                      rdf:type owl:FunctionalProperty ;
                      rdfs:domain :MusicTimeInterval ;
                      rdfs:range :MusicTimeDuration ;
                      owl:propertyDisjointWith :hasMusicTimeIndex ,
                                               :hasMusicTimeIndexComponent ,
                                               :hasMusicTimeInterval ,
                                               :hasSubject ,
                                               :hasValueType ,
                                               :includesObservation ,
                                               :isAnnotationTypeOf ,
                                               :isAnnotatorOf ,
                                               :isAnnotatorTypeOf ,
                                               :isJAMSAnnotationOf ,
                                               :isMusicTimeDurationOf ,
                                               :isMusicTimeIndexComponentOf ,
                                               :isMusicTimeIndexOf ,
                                               :isMusicTimeIntervalOf ,
                                               :isObservationOf ,
                                               :isValueTypeOf ;
                      rdfs:comment "Defines the relationship between a MusicTimeInterval and a MusicTimeDuration, defining the time duration of the interval."@en ;
                      rdfs:label "Has Music Time Duration"@en .


###  http://w3id.org/polifonia/ontology/jams/hasMusicTimeIndex
:hasMusicTimeIndex rdf:type owl:ObjectProperty ;
                   owl:inverseOf :isMusicTimeIndexOf ;
                   rdf:type owl:FunctionalProperty ;
                   rdfs:domain :MusicTimeInterval ;
                   rdfs:range :MusicTimeIndex ;
                   owl:propertyDisjointWith :hasMusicTimeIndexComponent ,
                                            :hasMusicTimeInterval ,
                                            :hasSubject ,
                                            :hasValueType ,
                                            :includesObservation ,
                                            :isAnnotationTypeOf ,
                                            :isAnnotatorOf ,
                                            :isAnnotatorTypeOf ,
                                            :isMusicTimeDurationOf ,
                                            :isMusicTimeIndexComponentOf ,
                                            :isMusicTimeIndexOf ,
                                            :isObservationOf ,
                                            :isValueTypeOf ;
                   rdfs:comment "Links a MusicTimeInterval to its MusicTimeIndex, which defines a point on the annotation/observation time sequence. It has two subclasses: hasEndMusicTimeIndex and hasStartMusicTimeIndex."@en ;
                   rdfs:label "Has Music Time Index"@en .


###  http://w3id.org/polifonia/ontology/jams/hasMusicTimeIndexComponent
:hasMusicTimeIndexComponent rdf:type owl:ObjectProperty ;
                            owl:inverseOf :isMusicTimeIndexComponentOf ;
                            rdf:type owl:InverseFunctionalProperty ;
                            rdfs:domain :MusicTimeIndex ;
                            rdfs:range :MusicTimeIndexComponent ;
                            owl:propertyDisjointWith :hasMusicTimeInterval ,
                                                     :hasSubject ,
                                                     :hasValueType ,
                                                     :includesObservation ,
                                                     :isAnnotationTypeOf ,
                                                     :isAnnotatorOf ,
                                                     :isAnnotatorTypeOf ,
                                                     :isMusicTimeDurationOf ,
                                                     :isMusicTimeIndexComponentOf ,
                                                     :isMusicTimeIndexOf ,
                                                     :isMusicTimeIntervalOf ,
                                                     :isObservationOf ,
                                                     :isValueTypeOf ;
                            rdfs:comment "Links a MusicTimeIndex to its/theirs MusicTimeIndexComponent, which represent the element(s) needed to describe a point on the timeline of the annotation/observation."@en ;
                            rdfs:label "Has Music Time Index Component"@en .


###  http://w3id.org/polifonia/ontology/jams/hasMusicTimeInterval
:hasMusicTimeInterval rdf:type owl:ObjectProperty ;
                      owl:inverseOf :isMusicTimeIntervalOf ;
                      rdf:type owl:FunctionalProperty ;
                      rdfs:domain [ rdf:type owl:Class ;
                                    owl:unionOf ( :JAMSAnnotation
                                                  :JAMSObservation
                                                )
                                  ] ;
                      rdfs:range :MusicTimeInterval ;
                      owl:propertyDisjointWith :hasSubject ,
                                               :hasValueType ,
                                               :includesObservation ,
                                               :isAnnotationTypeOf ,
                                               :isAnnotatorOf ,
                                               :isAnnotatorTypeOf ,
                                               :isJAMSAnnotationOf ,
                                               :isMusicTimeDurationOf ,
                                               :isMusicTimeIndexComponentOf ,
                                               :isMusicTimeIndexOf ,
                                               :isMusicTimeIntervalOf ,
                                               :isObservationOf ,
                                               :isValueTypeOf ;
                      rdfs:comment "Links a JAMSAnnotation or a JAMSObservation to its timing information, representaed by the class MusicTimeInterval."@en ;
                      rdfs:label "Has Music Time Interval"@en .


###  http://w3id.org/polifonia/ontology/jams/hasStartMusicTimeIndex
:hasStartMusicTimeIndex rdf:type owl:ObjectProperty ;
                        rdfs:subPropertyOf :hasMusicTimeIndex ,
                                           [ owl:inverseOf :isMusicTimeIndexOf
                                           ] ;
                        rdfs:domain :MusicTimeInterval ;
                        rdfs:range :MusicTimeIndex ;
                        rdfs:comment "Subproperty of jasMusicTimeIndex. It links a MusicTimeInterval to its MusicTimeIndex, defining the start point of validity of an observation/annotation time interval."@en ;
                        rdfs:label "Has Start Music Time Index"@en .


###  http://w3id.org/polifonia/ontology/jams/hasSubject
:hasSubject rdf:type owl:ObjectProperty ,
                     owl:FunctionalProperty ;
            rdfs:domain :JAMSObservation ;
            rdfs:range mr:MusicProjection ;
            owl:propertyDisjointWith :hasValueType ,
                                     :isAnnotatorOf ,
                                     :isAnnotatorTypeOf ,
                                     :isJAMSAnnotationOf ,
                                     :isMusicTimeDurationOf ,
                                     :isMusicTimeIndexComponentOf ,
                                     :isMusicTimeIndexOf ,
                                     :isMusicTimeIntervalOf ,
                                     :isObservationOf ,
                                     :isValueTypeOf ;
            rdfs:comment "Defines the subjecyt of a JAMSObservation, describing the type of value contained in the observation, described by the mf:MusicalFeature class."@en ;
            rdfs:label "Has Subject"@en .


###  http://w3id.org/polifonia/ontology/jams/hasValueType
:hasValueType rdf:type owl:ObjectProperty ;
              owl:inverseOf :isValueTypeOf ;
              rdf:type owl:FunctionalProperty ;
              rdfs:domain [ rdf:type owl:Class ;
                            owl:unionOf ( :MusicTimeDuration
                                          :MusicTimeIndexComponent
                                        )
                          ] ;
              rdfs:range :MusicTimeValueType ;
              owl:propertyDisjointWith :includesObservation ,
                                       :isAnnotationTypeOf ,
                                       :isJAMSAnnotationOf ,
                                       :isMusicTimeDurationOf ,
                                       :isMusicTimeIndexComponentOf ,
                                       :isMusicTimeIndexOf ,
                                       :isMusicTimeIntervalOf ,
                                       :isObservationOf ,
                                       :isValueTypeOf ;
              rdfs:comment "Links either a MusicTimeIndexComponent or a MusicTimeDuration to a MusicTimeValueType, defining the format in which the time information is expressed."@en ;
              rdfs:label "Has Music Time Value Type"@en .


###  http://w3id.org/polifonia/ontology/jams/includesObservation
:includesObservation rdf:type owl:ObjectProperty ;
                     owl:inverseOf :isObservationOf ;
                     rdf:type owl:InverseFunctionalProperty ;
                     rdfs:domain :JAMSAnnotation ;
                     rdfs:range :JAMSObservation ;
                     owl:propertyDisjointWith :isAnnotatorOf ,
                                              :isAnnotatorTypeOf ,
                                              :isJAMSAnnotationOf ,
                                              :isMusicTimeDurationOf ,
                                              :isMusicTimeIntervalOf ,
                                              :isObservationOf ;
                     rdfs:comment "Links a JAMS Annotation to the JAMS Onservation(s) it contains."@en ;
                     rdfs:label "Includes Observation"@en .


###  http://w3id.org/polifonia/ontology/jams/isAnnotationTypeOf
:isAnnotationTypeOf rdf:type owl:ObjectProperty ,
                             owl:InverseFunctionalProperty ;
                    rdfs:domain :AnnotationType ;
                    rdfs:range :JAMSAnnotation ;
                    owl:propertyDisjointWith :isAnnotatorTypeOf ,
                                             :isJAMSAnnotationOf ,
                                             :isMusicTimeDurationOf ,
                                             :isMusicTimeIndexComponentOf ,
                                             :isMusicTimeIntervalOf ,
                                             :isObservationOf ,
                                             :isValueTypeOf ;
                    rdfs:comment "Inverse of hasAnnotationType. Links an AnnotationType to a JAMSAnnotation."@en ;
                    rdfs:label "Is Annotation Type Of"@en .


###  http://w3id.org/polifonia/ontology/jams/isAnnotatorOf
:isAnnotatorOf rdf:type owl:ObjectProperty ;
               rdfs:range :JAMSAnnotation ;
               owl:propertyDisjointWith :isAnnotatorTypeOf ,
                                        :isJAMSAnnotationOf ,
                                        :isMusicTimeDurationOf ,
                                        :isMusicTimeIntervalOf ,
                                        :isObservationOf ,
                                        :isValueTypeOf ;
               rdfs:comment "Inverse of hasAnnotator. Links the Annotator to the JAMS Annotation annotated by such annotator."@en ;
               rdfs:label "Is Annotator Of"@en .


###  http://w3id.org/polifonia/ontology/jams/isAnnotatorTypeOf
:isAnnotatorTypeOf rdf:type owl:ObjectProperty ,
                            owl:InverseFunctionalProperty ;
                   rdfs:domain :AnnotatorType ;
                   owl:propertyDisjointWith :isJAMSAnnotationOf ,
                                            :isMusicTimeDurationOf ,
                                            :isMusicTimeIntervalOf ,
                                            :isObservationOf ;
                   rdfs:comment "Inverse of hasAnnotatorType. Links the Annotator Type to the Annotator class."@en ;
                   rdfs:label "Is Annotator Type Of"@en .


###  http://w3id.org/polifonia/ontology/jams/isJAMSAnnotationOf
:isJAMSAnnotationOf rdf:type owl:ObjectProperty ,
                             owl:FunctionalProperty ;
                    rdfs:domain :JAMSAnnotation ;
                    owl:propertyDisjointWith :isMusicTimeDurationOf ,
                                             :isMusicTimeIndexComponentOf ,
                                             :isMusicTimeIntervalOf ,
                                             :isObservationOf ;
                    rdfs:comment "Inverse of hasJAMSAnnotation. It links the JAMS Annotation to either a Recording o a Score."@en ;
                    rdfs:label "Is JAMS Annotation Of"@en .


###  http://w3id.org/polifonia/ontology/jams/isMusicTimeDurationOf
:isMusicTimeDurationOf rdf:type owl:ObjectProperty ,
                                owl:InverseFunctionalProperty ;
                       rdfs:domain :MusicTimeDuration ;
                       rdfs:range :MusicTimeInterval ;
                       owl:propertyDisjointWith :isMusicTimeIndexComponentOf ,
                                                :isMusicTimeIndexOf ,
                                                :isMusicTimeIntervalOf ,
                                                :isObservationOf ,
                                                :isValueTypeOf ;
                       rdfs:comment "Inverse of hasMusicTimeDuration. Links a MusicTimeDuration to the MusicTimeInterval it belongs to."@en ;
                       rdfs:label "Is Music Time Duration Of"@en .


###  http://w3id.org/polifonia/ontology/jams/isMusicTimeIndexComponentOf
:isMusicTimeIndexComponentOf rdf:type owl:ObjectProperty ,
                                      owl:FunctionalProperty ;
                             rdfs:domain :MusicTimeIndexComponent ;
                             rdfs:range :MusicTimeIndex ;
                             owl:propertyDisjointWith :isMusicTimeIndexOf ,
                                                      :isMusicTimeIntervalOf ,
                                                      :isObservationOf ,
                                                      :isValueTypeOf ;
                             rdfs:comment "Inverse of hasMusicTimeIndexComponent. Defines the relation between a MusicTimeIndexComponent and the MusicITimeIndex it belongs to."@en ;
                             rdfs:label "Is Music Time Index Component Of"@en .


###  http://w3id.org/polifonia/ontology/jams/isMusicTimeIndexOf
:isMusicTimeIndexOf rdf:type owl:ObjectProperty ,
                             owl:InverseFunctionalProperty ;
                    rdfs:domain :MusicTimeIndex ;
                    rdfs:range :MusicTimeInterval ;
                    owl:propertyDisjointWith :isMusicTimeIntervalOf ,
                                             :isObservationOf ,
                                             :isValueTypeOf ;
                    rdfs:comment "Inverse of hasMusicTimeIndex. It links a MusicTimeIndex with the MusicTimeInterval it belongs to."@en ;
                    rdfs:label "Is Music Time Index Of"@en .


###  http://w3id.org/polifonia/ontology/jams/isMusicTimeIntervalOf
:isMusicTimeIntervalOf rdf:type owl:ObjectProperty ,
                                owl:InverseFunctionalProperty ;
                       rdfs:domain :MusicTimeInterval ;
                       rdfs:range [ rdf:type owl:Class ;
                                    owl:unionOf ( :JAMSAnnotation
                                                  :JAMSObservation
                                                )
                                  ] ;
                       owl:propertyDisjointWith :isObservationOf ,
                                                :isValueTypeOf ;
                       rdfs:comment "Inverse of hasMusicTimeInterval. It links a MusicTimeInterval to a JAMSAnnotation or to a JAMSObservation."@en ;
                       rdfs:label "Is Music Time Interval Of"@en .


###  http://w3id.org/polifonia/ontology/jams/isObservationOf
:isObservationOf rdf:type owl:ObjectProperty ,
                          owl:FunctionalProperty ;
                 rdfs:domain :JAMSObservation ;
                 rdfs:range :JAMSAnnotation ;
                 owl:propertyDisjointWith :isValueTypeOf ;
                 rdfs:comment "Inverse of includesObservation. Links a JAMS Observation to the JAMS Annotation to which it belongs."@en ;
                 rdfs:label "Is Observation Of"@en .


###  http://w3id.org/polifonia/ontology/jams/isValueTypeOf
:isValueTypeOf rdf:type owl:ObjectProperty ,
                        owl:InverseFunctionalProperty ;
               rdfs:domain :MusicTimeValueType ;
               rdfs:range [ rdf:type owl:Class ;
                            owl:unionOf ( :MusicTimeDuration
                                          :MusicTimeIndexComponent
                                        )
                          ] ;
               rdfs:comment "Inverse of hasMusicTimeValueType. Links a MusicValueType either to a MusicTimeIndexComonent or to a MusicTimeDuration."@en ;
               rdfs:label "Is Music Time Value Type Of"@en .


###  http://www.w3.org/ns/prov#WasDerivedFrom
prov:WasDerivedFrom rdf:type owl:ObjectProperty ;
                    rdfs:domain [ rdf:type owl:Class ;
                                  owl:unionOf ( :JAMSAnnotation
                                                :JAMSFile
                                              )
                                ] ;
                    rdfs:label "Was Derived From"@en .


###  http://www.w3.org/ns/prov#wasMemberOf
prov:wasMemberOf rdf:type owl:ObjectProperty ;
                 rdfs:domain :JAMSFile ;
                 rdfs:label "Was Member Of"@en .


#################################################################
#    Data properties
#################################################################

###  http://w3id.org/polifonia/ontology/jams/hasConfidence
:hasConfidence rdf:type owl:DatatypeProperty ,
                        owl:FunctionalProperty ;
               rdfs:domain :JAMSObservation ;
               rdfs:range xsd:float ;
               owl:propertyDisjointWith :hasName ,
                                        :hasValue ;
               rdfs:comment "The confidence of an annotation/observation, as described by the JAMS documentation, hence expressed with a floating number from 0 to 1."@en ;
               rdfs:label "Has Confidence"@en .


###  http://w3id.org/polifonia/ontology/jams/hasName
:hasName rdf:type owl:DatatypeProperty ;
         rdfs:range xsd:string ;
         owl:propertyDisjointWith :hasValue ;
         rdfs:comment "The name of an annotator, which can be either human, artificial (e.g. the name of a software) or describing a group of people (e.g. the name of a crowdsourcing service/event)."@en ;
         rdfs:label "Has Name"@en .


###  http://w3id.org/polifonia/ontology/jams/hasValue
:hasValue rdf:type owl:DatatypeProperty ,
                   owl:FunctionalProperty ;
          rdfs:domain [ rdf:type owl:Class ;
                        owl:unionOf ( :MusicTimeDuration
                                      :MusicTimeIndexComponent
                                    )
                      ] ;
          rdfs:range rdfs:Literal ;
          rdfs:comment "Defines the time value of either a MusicTimeIndexComponent or a MusicTimeDuration."@en ;
          rdfs:label "Has Value"@en .


#################################################################
#    Classes
#################################################################

###  http://w3id.org/polifonia/ontology/jams/AnnotationType
:AnnotationType rdf:type owl:Class ;
                rdfs:subClassOf [ rdf:type owl:Restriction ;
                                  owl:onProperty :isAnnotationTypeOf ;
                                  owl:allValuesFrom :JAMSAnnotation
                                ] ;
                owl:disjointWith :AnnotatorType ,
                                 :File ,
                                 :Format ,
                                 :JAMSAnnotation ,
                                 :JAMSObservation ,
                                 :MusicTimeDuration ,
                                 :MusicTimeIndex ,
                                 :MusicTimeIndexComponent ,
                                 :MusicTimeInterval ,
                                 :MusicTimeValueType ;
                rdfs:label "Annotation Type"@en ,
                           "The type of the annotation. It maps directly to the annotation's \"namespace\" of a JAMS file."@en .


###  http://w3id.org/polifonia/ontology/jams/AnnotatorType
:AnnotatorType rdf:type owl:Class ;
               owl:disjointWith :File ,
                                :Format ,
                                :JAMSAnnotation ,
                                :JAMSFile ,
                                :JAMSObservation ,
                                :MusicTimeDuration ,
                                :MusicTimeIndex ,
                                :MusicTimeIndexComponent ,
                                :MusicTimeInterval ,
                                :MusicTimeValueType ;
               rdfs:comment "The type of annotator of a JAMS annotation, whether human or the result of an automatic or crowdsourced annotation."@en ;
               rdfs:label "Annotator Type"@en .


###  http://w3id.org/polifonia/ontology/jams/File
:File rdf:type owl:Class ;
      rdfs:subClassOf [ rdf:type owl:Restriction ;
                        owl:onProperty :hasFormat ;
                        owl:allValuesFrom :Format
                      ] ,
                      [ rdf:type owl:Restriction ;
                        owl:onProperty :hasFormat ;
                        owl:hasValue <http://w3id.org/polifonia/resource/Format/jams>
                      ] ;
      owl:disjointWith :Format ,
                       :JAMSAnnotation ,
                       :JAMSObservation ,
                       :MusicTimeDuration ,
                       :MusicTimeIndex ,
                       :MusicTimeIndexComponent ,
                       :MusicTimeInterval ,
                       :MusicTimeValueType ;
      rdfs:comment "Any type of file"@en ;
      rdfs:label "File"@en .


###  http://w3id.org/polifonia/ontology/jams/Format
:Format rdf:type owl:Class ;
        owl:disjointWith :JAMSAnnotation ,
                         :JAMSObservation ,
                         :MusicTimeDuration ,
                         :MusicTimeIndex ,
                         :MusicTimeIndexComponent ,
                         :MusicTimeInterval ,
                         :MusicTimeValueType ;
        rdfs:comment "Format of files e.g. .jams, .doc, .xml"@en ;
        rdfs:label "Format"@en .


###  http://w3id.org/polifonia/ontology/jams/JAMSAnnotation
:JAMSAnnotation rdf:type owl:Class ;
                rdfs:subClassOf [ rdf:type owl:Restriction ;
                                  owl:onProperty :hasAnnotationType ;
                                  owl:allValuesFrom :AnnotationType
                                ] ,
                                [ rdf:type owl:Restriction ;
                                  owl:onProperty :hasMusicTimeInterval ;
                                  owl:allValuesFrom :MusicTimeInterval
                                ] ,
                                [ rdf:type owl:Restriction ;
                                  owl:onProperty :includesObservation ;
                                  owl:allValuesFrom :JAMSObservation
                                ] ,
                                [ rdf:type owl:Restriction ;
                                  owl:onProperty prov:WasDerivedFrom ;
                                  owl:allValuesFrom :JAMSFile
                                ] ,
                                [ rdf:type owl:Restriction ;
                                  owl:onProperty :hasAnnotationType ;
                                  owl:qualifiedCardinality "1"^^xsd:nonNegativeInteger ;
                                  owl:onClass :AnnotationType
                                ] ,
                                [ rdf:type owl:Restriction ;
                                  owl:onProperty :hasMusicTimeInterval ;
                                  owl:qualifiedCardinality "1"^^xsd:nonNegativeInteger ;
                                  owl:onClass :MusicTimeInterval
                                ] ;
                owl:disjointWith :JAMSFile ,
                                 :JAMSObservation ,
                                 :MusicTimeDuration ,
                                 :MusicTimeIndex ,
                                 :MusicTimeIndexComponent ,
                                 :MusicTimeInterval ;
                rdfs:comment "A group of observations that share the same type of annotation (e.g. score or audio) and the same syntax with which the agreement is expressed (e.g. Harte or Roman)."@en ;
                rdfs:label "JAMS Annotation"@en .


###  http://w3id.org/polifonia/ontology/jams/JAMSAudioAnnotation
:JAMSAudioAnnotation rdf:type owl:Class ;
                     rdfs:subClassOf :JAMSAnnotation ,
                                     [ rdf:type owl:Restriction ;
                                       owl:onProperty :includesObservation ;
                                       owl:allValuesFrom :JAMSAudioObservation
                                     ] ;
                     owl:disjointWith :JAMSScoreAnnotation ;
                     rdfs:comment "An annotation describing a piece of music annotated on the basis of an audio track."@en ;
                     rdfs:label "JAMS Audio Annotation"@en .


###  http://w3id.org/polifonia/ontology/jams/JAMSAudioObservation
:JAMSAudioObservation rdf:type owl:Class ;
                      rdfs:subClassOf :JAMSObservation ,
                                      [ rdf:type owl:Restriction ;
                                        owl:onProperty :isObservationOf ;
                                        owl:allValuesFrom :JAMSAudioAnnotation
                                      ] ,
                                      [ rdf:type owl:Restriction ;
                                        owl:onProperty :isObservationOf ;
                                        owl:qualifiedCardinality "1"^^xsd:nonNegativeInteger ;
                                        owl:onClass :JAMSAudioAnnotation
                                      ] ;
                      owl:disjointWith :JAMSScoreObservation ;
                      rdfs:comment "A observation defined on the audio signal, i.e. described from a temporal point of view using real time, usually expressed in seconds."@en ;
                      rdfs:label "JAMS Audio Observation"@en .


###  http://w3id.org/polifonia/ontology/jams/JAMSFile
:JAMSFile rdf:type owl:Class ;
          rdfs:subClassOf :File ;
          owl:disjointWith :JAMSObservation ;
          rdfs:comment "A file in JAMS format (with extension .jams, a serialisation of JSON), containing musical annotations structured according to JAMS specifications."@en ;
          rdfs:label "The class of files encoded in JAMS format (JAMS is a datamodel serialised in a json-specific format)."@en .


###  http://w3id.org/polifonia/ontology/jams/JAMSObservation
:JAMSObservation rdf:type owl:Class ;
                 rdfs:subClassOf [ rdf:type owl:Restriction ;
                                   owl:onProperty :hasMusicTimeInterval ;
                                   owl:allValuesFrom :MusicTimeInterval
                                 ] ,
                                 [ rdf:type owl:Restriction ;
                                   owl:onProperty :isObservationOf ;
                                   owl:allValuesFrom :JAMSAnnotation
                                 ] ,
                                 [ rdf:type owl:Restriction ;
                                   owl:onProperty :hasMusicTimeInterval ;
                                   owl:qualifiedCardinality "1"^^xsd:nonNegativeInteger ;
                                   owl:onClass :MusicTimeInterval
                                 ] ,
                                 [ rdf:type owl:Restriction ;
                                   owl:onProperty :isObservationOf ;
                                   owl:qualifiedCardinality "1"^^xsd:nonNegativeInteger ;
                                   owl:onClass :JAMSAnnotation
                                 ] ,
                                 [ rdf:type owl:Restriction ;
                                   owl:onProperty :hasConfidence ;
                                   owl:allValuesFrom xsd:float
                                 ] ,
                                 [ rdf:type owl:Restriction ;
                                   owl:onProperty :hasConfidence ;
                                   owl:qualifiedCardinality "1"^^xsd:nonNegativeInteger ;
                                   owl:onDataRange xsd:float
                                 ] ;
                 owl:disjointWith :MusicTimeDuration ,
                                  :MusicTimeIndex ,
                                  :MusicTimeIndexComponent ,
                                  :MusicTimeInterval ,
                                  :MusicTimeValueType ;
                 rdfs:comment "An observation of the annotation, understood as an event defined in time (both real and symbolic) that has a value (e.g. a specific agreement) and a precise duration."@en ;
                 rdfs:label "JAMS Observation"@en .


###  http://w3id.org/polifonia/ontology/jams/JAMSScoreAnnotation
:JAMSScoreAnnotation rdf:type owl:Class ;
                     rdfs:subClassOf :JAMSAnnotation ,
                                     [ rdf:type owl:Restriction ;
                                       owl:onProperty :includesObservation ;
                                       owl:allValuesFrom :JAMSScoreObservation
                                     ] ;
                     rdfs:comment "An annotation describing a piece of music annotated on the basis of a music score."@en ;
                     rdfs:label "JAMS Score Annotation"@en .


###  http://w3id.org/polifonia/ontology/jams/JAMSScoreObservation
:JAMSScoreObservation rdf:type owl:Class ;
                      rdfs:subClassOf :JAMSObservation ,
                                      [ rdf:type owl:Restriction ;
                                        owl:onProperty :isObservationOf ;
                                        owl:allValuesFrom :JAMSScoreAnnotation
                                      ] ,
                                      [ rdf:type owl:Restriction ;
                                        owl:onProperty :isObservationOf ;
                                        owl:qualifiedCardinality "1"^^xsd:nonNegativeInteger ;
                                        owl:onClass :JAMSScoreAnnotation
                                      ] ;
                      rdfs:comment "A observation defined on a symbolic notation or on a music score, i.e. described from a temporal point of view using references to symbolic elements defined by the notation itself."@en ;
                      rdfs:label "JAMS Score Observation"@en .


###  http://w3id.org/polifonia/ontology/jams/MusicTimeDuration
:MusicTimeDuration rdf:type owl:Class ;
                   rdfs:subClassOf [ rdf:type owl:Restriction ;
                                     owl:onProperty :hasValueType ;
                                     owl:allValuesFrom :MusicTimeValueType
                                   ] ,
                                   [ rdf:type owl:Restriction ;
                                     owl:onProperty :isMusicTimeDurationOf ;
                                     owl:allValuesFrom :MusicTimeInterval
                                   ] ,
                                   [ rdf:type owl:Restriction ;
                                     owl:onProperty :hasValueType ;
                                     owl:qualifiedCardinality "1"^^xsd:nonNegativeInteger ;
                                     owl:onClass :MusicTimeValueType
                                   ] ,
                                   [ rdf:type owl:Restriction ;
                                     owl:onProperty :hasValue ;
                                     owl:someValuesFrom rdfs:Literal
                                   ] ,
                                   [ rdf:type owl:Restriction ;
                                     owl:onProperty :hasValue ;
                                     owl:cardinality "1"^^xsd:nonNegativeInteger
                                   ] ;
                   owl:disjointWith :MusicTimeIndex ,
                                    :MusicTimeIndexComponent ,
                                    :MusicTimeInterval ,
                                    :MusicTimeValueType ;
                   rdfs:comment "The duration of a MusicTimeInterval, which defines a value and a ValueType."@en ;
                   rdfs:label "Music Time Duration"@en .


###  http://w3id.org/polifonia/ontology/jams/MusicTimeIndex
:MusicTimeIndex rdf:type owl:Class ;
                rdfs:subClassOf [ rdf:type owl:Restriction ;
                                  owl:onProperty :hasMusicTimeIndexComponent ;
                                  owl:allValuesFrom :MusicTimeIndexComponent
                                ] ,
                                [ rdf:type owl:Restriction ;
                                  owl:onProperty :isMusicTimeIndexOf ;
                                  owl:allValuesFrom :MusicTimeInterval
                                ] ,
                                [ rdf:type owl:Restriction ;
                                  owl:onProperty :hasMusicTimeIndexComponent ;
                                  owl:minQualifiedCardinality "1"^^xsd:nonNegativeInteger ;
                                  owl:onClass :MusicTimeIndexComponent
                                ] ;
                owl:disjointWith :MusicTimeIndexComponent ,
                                 :MusicTimeInterval ,
                                 :MusicTimeValueType ;
                rdfs:comment "An index that defines a point in a musical sequence, whether it is a temporal sequence (expressed in real time) or a symbolic sequence (expressed in symbolic time)."@en ;
                rdfs:label "Music Time Index"@en .


###  http://w3id.org/polifonia/ontology/jams/MusicTimeIndexComponent
:MusicTimeIndexComponent rdf:type owl:Class ;
                         rdfs:subClassOf [ rdf:type owl:Restriction ;
                                           owl:onProperty :hasValueType ;
                                           owl:allValuesFrom :MusicTimeValueType
                                         ] ,
                                         [ rdf:type owl:Restriction ;
                                           owl:onProperty :isMusicTimeIndexComponentOf ;
                                           owl:allValuesFrom :MusicTimeIndex
                                         ] ,
                                         [ rdf:type owl:Restriction ;
                                           owl:onProperty :hasValueType ;
                                           owl:qualifiedCardinality "1"^^xsd:nonNegativeInteger ;
                                           owl:onClass :MusicTimeValueType
                                         ] ,
                                         [ rdf:type owl:Restriction ;
                                           owl:onProperty :hasValue ;
                                           owl:someValuesFrom rdfs:Literal
                                         ] ,
                                         [ rdf:type owl:Restriction ;
                                           owl:onProperty :hasValue ;
                                           owl:cardinality "1"^^xsd:nonNegativeInteger
                                         ] ;
                         owl:disjointWith :MusicTimeInterval ,
                                          :MusicTimeValueType ;
                         rdfs:comment "A component of a MusicTimeIndex, which defines the value of the component and its ValueType. Multiple MusicTimeIndexComponents are required for representing points on a sequence that requires more than one value to be defined. For example, a symbolic notation usually needs beats and measures to define a point on a sequence: in this case there will be a MusicTimeIndexComponents defining the measure position and another MusicTimeIndexComponents for defining the beat position."@en ;
                         rdfs:label "Music Time Index Comonent"@en .


###  http://w3id.org/polifonia/ontology/jams/MusicTimeInterval
:MusicTimeInterval rdf:type owl:Class ;
                   rdfs:subClassOf [ rdf:type owl:Restriction ;
                                     owl:onProperty :isMusicTimeIntervalOf ;
                                     owl:someValuesFrom [ rdf:type owl:Class ;
                                                          owl:unionOf ( :JAMSAnnotation
                                                                        :JAMSObservation
                                                                      )
                                                        ]
                                   ] ,
                                   [ rdf:type owl:Restriction ;
                                     owl:onProperty :hasMusicTimeDuration ;
                                     owl:allValuesFrom :MusicTimeDuration
                                   ] ,
                                   [ rdf:type owl:Restriction ;
                                     owl:onProperty :hasMusicTimeIndex ;
                                     owl:allValuesFrom :MusicTimeIndex
                                   ] ,
                                   [ rdf:type owl:Restriction ;
                                     owl:onProperty :hasMusicTimeIndex ;
                                     owl:minQualifiedCardinality "1"^^xsd:nonNegativeInteger ;
                                     owl:onClass :MusicTimeIndex
                                   ] ,
                                   [ rdf:type owl:Restriction ;
                                     owl:onProperty :hasMusicTimeDuration ;
                                     owl:qualifiedCardinality "1"^^xsd:nonNegativeInteger ;
                                     owl:onClass :MusicTimeDuration
                                   ] ;
                   owl:disjointWith :MusicTimeValueType ;
                   rdfs:comment "The interval in which an Annotation or an Observation takes place. It describe the time frame in which the Annotation/Observation is valid."@en ;
                   rdfs:label "Music Time Interval"@en .


###  http://w3id.org/polifonia/ontology/jams/MusicTimeValueType
:MusicTimeValueType rdf:type owl:Class ;
                    rdfs:subClassOf [ rdf:type owl:Restriction ;
                                      owl:onProperty :isValueTypeOf ;
                                      owl:someValuesFrom :MusicTimeDuration
                                    ] ,
                                    [ rdf:type owl:Restriction ;
                                      owl:onProperty :isValueTypeOf ;
                                      owl:someValuesFrom :MusicTimeIndexComponent
                                    ] ;
                    rdfs:comment "It defines the type of the temporal value being represented, for example seconds for audio annotations and beat/measure for score annotations."@en ;
                    rdfs:label "Music Time Value Type"@en .


###  http://www.w3.org/1999/02/22-rdf-syntax-ns#List
rdf:List rdf:type owl:Class .


###  https://w3id.org/polifonia/ontology/music-representation/MusicContent
mr:MusicContent owl:equivalentClass [ rdf:type owl:Class ;
                                      owl:unionOf ( mm:AbstractScore
                                                    mm:Recording
                                                    mm:Score
                                                  )
                                    ] .


#################################################################
#    Individuals
#################################################################

###  http://w3id.org/polifonia/resource/AnnotationType/chord
<http://w3id.org/polifonia/resource/AnnotationType/chord> rdf:type owl:NamedIndividual ,
                                                                   :AnnotationType ;
                                                          rdfs:label "Chord"@en .


###  http://w3id.org/polifonia/resource/AnnotationType/chord_harte
<http://w3id.org/polifonia/resource/AnnotationType/chord_harte> rdf:type owl:NamedIndividual ,
                                                                         :AnnotationType ;
                                                                rdfs:label "Chord Harte"@en .


###  http://w3id.org/polifonia/resource/AnnotationType/chord_roman
<http://w3id.org/polifonia/resource/AnnotationType/chord_roman> rdf:type owl:NamedIndividual ,
                                                                         :AnnotationType ;
                                                                rdfs:label "Chord Roman"@en .


###  http://w3id.org/polifonia/resource/AnnotationType/key_mode
<http://w3id.org/polifonia/resource/AnnotationType/key_mode> rdf:type owl:NamedIndividual ,
                                                                      :AnnotationType ;
                                                             rdfs:label "Key Mode"@en .


###  http://w3id.org/polifonia/resource/AnnotatorType/crowd
<http://w3id.org/polifonia/resource/AnnotatorType/crowd> rdf:type owl:NamedIndividual ,
                                                                  :AnnotatorType ;
                                                         rdfs:comment "Then annotations are obtained through crowdsourcing the agent producing them is the crowd"@en ;
                                                         rdfs:label "Crowd"@en .


###  http://w3id.org/polifonia/resource/AnnotatorType/expert_human
<http://w3id.org/polifonia/resource/AnnotatorType/expert_human> rdf:type owl:NamedIndividual ,
                                                                         :AnnotatorType ;
                                                                rdfs:comment "Expert Human"@en .


###  http://w3id.org/polifonia/resource/AnnotatorType/program
<http://w3id.org/polifonia/resource/AnnotatorType/program> rdf:type owl:NamedIndividual ,
                                                                    :AnnotatorType ;
                                                           rdfs:label "Program"@en .


###  http://w3id.org/polifonia/resource/Format/jams
<http://w3id.org/polifonia/resource/Format/jams> rdf:type owl:NamedIndividual ,
                                                          :Format ;
                                                 rdfs:label "JAMS"@en .


###  http://w3id.org/polifonia/resource/MusicTimeValueType/beat
<http://w3id.org/polifonia/resource/MusicTimeValueType/beat> rdf:type owl:NamedIndividual ,
                                                                      :MusicTimeValueType ;
                                                             rdfs:label "Beat"@en .


###  http://w3id.org/polifonia/resource/MusicTimeValueType/measure
<http://w3id.org/polifonia/resource/MusicTimeValueType/measure> rdf:type owl:NamedIndividual ,
                                                                         :MusicTimeValueType ;
                                                                rdfs:label "Measure"@en .


###  http://w3id.org/polifonia/resource/MusicTimeValueType/second
<http://w3id.org/polifonia/resource/MusicTimeValueType/second> rdf:type owl:NamedIndividual ,
                                                                        :MusicTimeValueType ;
                                                               rdfs:label "Second"@en .


###  Generated by the OWL API (version 4.5.9.2019-02-01T07:24:44Z) https://github.com/owlcs/owlapi
